coq-semws11.v
@@ -433,7 +433,10 @@ Lemma R_term_ap : forall S T t,
   ~value t ->
   E (tyA S T) t ->
   forall s, R S s -> R T (tmA t s).
-intros S T t H0 H1 H2 H3 s H4. generalize (R_ter S s H4). intros H. revert H4. induction H as [s H IH].
+Proof.  
+  intros S T t H0 H1 H2 H3 s H4. generalize (R_ter S s H4). intros H. revert H4.
+  unfold ter in H. 
+  induction H as [s H IH].
 intros H4. apply H0.
 econstructor. eassumption. apply R_typed. assumption.
 intros H5. inv H5.
@@ -457,7 +460,7 @@ Proof.
   apply H3. assumption.
   - intros t H1 H2 H3. simpl. do 2 (try split).
     + assumption.
-    + constructor. intros t' H4. apply R_ter with (T := (tyA T1 T2)).
+    + unfold E in H3. constructor. intros t' H4. apply R_ter with (T := (tyA T1 T2)).
       apply H3. assumption.
     + intros s H4. apply (R_term_ap IHT2 H1 H2 H3).
       assumption.
@@ -466,14 +469,15 @@ Qed.
 Lemma R_beta : forall S T x t, type (update empty x S) t T ->
   (forall s, R S s -> R T (subst x s t)) ->
   forall s, R S s -> R T (tmA (tmL x S t) s).
-intros S T x t H0 H1 s H2. generalize (R_ter S s H2). intros H. revert H2. induction H. intros H3.
-apply R_exp_closed.
-econstructor. econstructor. assumption. apply R_typed. assumption.
-intros H4. inv H4.
-intros t' H4. inv H4.
-apply H1. assumption.
-inv H8.
-apply H2. assumption. apply R_step_closed with (t := x0); assumption.
+Proof.
+  intros S T x t H0 H1 s H2. generalize (R_ter S s H2). intros H. revert H2. induction H. intros H3.
+  apply R_exp_closed.
+  econstructor. econstructor. assumption. apply R_typed. assumption.
+  intros H4. inv H4.
+  intros t' H4. inv H4.
+  apply H1. assumption.
+  inv H8.
+  apply H2. assumption. apply R_step_closed with (t := x0); assumption.
 Qed.
 
 
